new/proof/github_com/sanjit_bhat/pav/server_proof/server.v
@@ -1,14 +1,25 @@
 From New.generatedproof.github_com.sanjit_bhat.pav Require Import server.
 From New.proof.github_com.sanjit_bhat.pav Require Import prelude.
 
-(*
+From New.proof Require Import sync time.
+From New.proof.github_com.goose_lang Require Import std.
 From New.proof.github_com.sanjit_bhat.pav Require Import
-  advrpc auditor cryptoffi hashchain ktcore merkle server sigpred. *)
+  cryptoffi hashchain ktcore merkle.
 
 Module server.
 
+Module state.
+Record t :=
+  mk {
+    (* gmap from uid's to list of pks (indexed by version). *)
+    keys: gmap w64 (list $ list w8);
+    digs: list $ list w8;
+  }.
+End state.
+
 Section proof.
 Context `{hG: heapGS Σ, !ffi_semantics _ _, !globalsGS Σ} {go_ctx : GoContext}.
+Context `{!pavG Σ}.
 
 Axiom Server_names : Type.
 
@@ -17,40 +28,52 @@ Implicit Types γ : Server_names.
 
 Axiom is_Server : ∀ (s : loc) γ, iProp Σ.
 
-Definition state := gmap Z Z.
-
-Axiom own_Server : ∀ γ (σ : state), iProp Σ.
+Axiom own_Server : ∀ γ (σ : state.t), iProp Σ.
 
 Axiom own_Server_timeless : ∀ γ σ,  Timeless (own_Server γ σ).
 Global Existing Instance own_Server_timeless.
 
-Axiom pure_put : w64 → list w8 → w64 → state → state.
+Axiom pure_put : w64 → list w8 → w64 → state.t → state.t.
 
-(* Rpc spec needs □ in front of atomic update. *)
-Lemma wp_Server__Put s γ uid pk pk_sl ver :
+(* RPC spec needs □ in front of atomic update. *)
+Lemma wp_Server_Put s γ uid pk sl_pk ver :
   ∀ Φ,
   is_Server s γ -∗
-  pk_sl ↦* pk -∗
-  (|={⊤,∅}=> ∃ σ, own_Server γ σ ∗
-        (own_Server γ (pure_put uid pk ver σ) ={∅,⊤}=∗ True)) -∗
-  Φ #() -∗
-  WP s @ (ptrT.id server.Server.id) @ "Put" #uid #pk_sl #ver {{ Φ }}.
+  sl_pk ↦*□ pk -∗
+  □ (|={⊤,∅}=> ∃ σ, own_Server γ σ ∗
+    (own_Server γ (pure_put uid pk ver σ) ={∅,⊤}=∗
+      Φ #())) -∗
+  WP s @ (ptrT.id server.Server.id) @ "Put" #uid #sl_pk #ver {{ Φ }}.
 Proof.
 Admitted.
 
-Axiom pure_history :
-  ∀ (uid prevEpoch prevVerLen : w64) (σ : state), val.
-  (* (list w8 * list w8 * list ktcore.Memb.t * ktcore.NonMemb.t * ktcore.Blame.t). *)
-
-Axiom CRYPTO_FACTS : iProp Σ.
-
-(* The RPC spec is the same, no □ because this doesn't mutate σ. *)
-Lemma wp_Server__History s γ uid prevEpoch prevVerLen :
+(* The RPC spec is the same, no □ bc this doesn't mutate σ. *)
+(* for idiomatic spec, use GS to contradict BlameUnknown. *)
+Lemma wp_Server_History s γ (uid prevEpoch prevVerLen : w64) :
   ∀ Φ,
   is_Server s γ -∗
-  (|={⊤,∅}=> ∃ σ, own_Server γ σ ∗
-        (own_Server γ σ ={∅,⊤}=∗
-         CRYPTO_FACTS -∗ Φ (pure_history uid prevEpoch prevVerLen σ))) -∗
+  (|={⊤,∅}=> ∃ σ, own_Server γ σ ∗ (own_Server γ σ ={∅,⊤}=∗
+    (* postcond. *)
+    ∃ (sl_chainProof sl_linkSig sl_hist : slice.t) (ptr_bound : loc) (err : ktcore.Blame),
+    ((
+      "%Herr" ∷ ⌜err = {[ ktcore.BlameUnknown ]}⌝ ∗
+      "%Hwish" ∷ ⌜uint.nat prevEpoch ≥ length σ.(state.digs) ∨
+        uint.nat prevVerLen > length (σ.(state.keys) !!! uid)⌝
+    ) ∨ (
+      ∃ chainProof (linkSig : list w8) sl0_hist hist bound,
+      "%Herr" ∷ ⌜err = ∅⌝ ∗
+
+      "#Hsl_chainProof" ∷ sl_chainProof ↦*□ chainProof ∗
+      "#Hsl_linkSig" ∷ sl_linkSig ↦*□ linkSig ∗
+      "#Hsl_hist" ∷ sl_hist ↦*□ sl0_hist ∗
+      "#Hsl0_hist" ∷ ([∗ list] ptr;obj ∈ sl0_hist;hist,
+        ktcore.Memb.own ptr obj (□)) ∗
+      "#Hptr_bound" ∷ ktcore.NonMemb.own ptr_bound bound (□) ∗
+
+      "%Hwish_chainProof" ∷ ⌜hashchain.wish_Verify chainProof
+        (drop (S (uint.nat prevEpoch)) σ.(state.digs))⌝)) -∗
+      (* TODO: correctness preds should tie into σ. *)
+    Φ #(sl_chainProof, sl_linkSig, sl_hist, ptr_bound, err))) -∗
   WP s @ (ptrT.id server.Server.id) @ "History" #uid #prevEpoch #prevVerLen {{ Φ }}.
 Proof.
 Admitted.
@@ -65,5 +88,6 @@ inv (∃ σ,
 
 (* For proving the "adversarial clients" idiom spec, perhaps only need an invariant
    like: inv (∃ σ, own_Server γs σ) *)
+
 End proof.
 End server.
